Merkle tree: proved the invariants of flushing in high-level design

secure_api/merkle_tree/MerkleTree.New.High.Correct.fst
@@ -173,6 +173,21 @@ let rec merge_hs_slice_equal ahs1 ahs2 bhs1 bhs2 i j =
        assert (S.index ahs2 i == S.index bhs2 i);
        merge_hs_slice_equal ahs1 ahs2 bhs1 bhs2 (i + 1) j)
 
+val merge_hs_upd:
+  hs1:hash_ss ->
+  hs2:hash_ss{S.length hs1 = S.length hs2} ->
+  i:nat{i < S.length hs1} ->
+  v1:hash_seq -> v2:hash_seq ->
+  Lemma (requires (S.equal (S.append (S.index hs1 i) (S.index hs2 i))
+                           (S.append v1 v2)))
+        (ensures (S.equal (merge_hs hs1 hs2)
+                          (merge_hs (S.upd hs1 i v1) (S.upd hs2 i v2))))
+        (decreases i)
+let rec merge_hs_upd hs1 hs2 i v1 v2 =
+  if S.length hs1 = 0 then ()
+  else if i = 0 then ()
+  else merge_hs_upd (S.tail hs1) (S.tail hs2) (i - 1) v1 v2
+
 val mt_olds_inv:
   lv:nat{lv <= 32} ->
   i:nat ->
@@ -183,6 +198,20 @@ let rec mt_olds_inv lv i olds =
   else (let ofs = offset_of i in
        S.length (S.index olds lv) == ofs /\
        mt_olds_inv (lv + 1) (i / 2) olds)
+
+val mt_olds_inv_equiv:
+  lv:nat{lv <= 32} ->
+  i:nat ->
+  olds1:hash_ss{S.length olds1 = 32} ->
+  olds2:hash_ss{S.length olds2 = 32} ->
+  Lemma (requires (mt_olds_inv lv i olds1 /\
+                  S.equal (S.slice olds1 lv 32) (S.slice olds2 lv 32)))
+        (ensures (mt_olds_inv lv i olds2))
+        (decreases (32 - lv))
+let rec mt_olds_inv_equiv lv i olds1 olds2 =
+  if lv = 32 then ()
+  else (assert (S.index olds1 lv == S.index olds2 lv);
+       mt_olds_inv_equiv (lv + 1) (i / 2) olds1 olds2)
 
 val mt_olds_hs_lth_inv_ok:
   lv:nat{lv <= 32} ->
@@ -317,7 +346,7 @@ val insert_inv_preserved:
   Lemma (requires (mt_olds_hs_inv lv i j olds hs))
         (ensures (mt_olds_hs_inv lv i (j + 1) olds (insert_ lv i j hs acc)))
         (decreases (32 - lv))
-#reset-options "--z3rlimit 80 --max_fuel 2"
+#reset-options "--z3rlimit 160 --max_fuel 2"
 let rec insert_inv_preserved lv i j olds hs acc =
   if j % 2 = 1 
   then begin
@@ -361,6 +390,7 @@ let rec insert_inv_preserved lv i j olds hs acc =
     insert_inv_preserved_even lv i j olds hs acc;
     assert (mt_olds_hs_inv lv i (j + 1) olds (insert_ lv i j hs acc))
   end
+#reset-options
 
 val mt_insert_inv_preserved:
   mt:merkle_tree{mt_wf_elts mt /\ mt_not_full mt} -> v:hash ->
@@ -370,9 +400,140 @@ val mt_insert_inv_preserved:
 let mt_insert_inv_preserved mt v olds =
   insert_inv_preserved 0 (MT?.i mt) (MT?.j mt) olds (MT?.hs mt) v
 
-/// Correctness of `mt_get_root` and `mt_get_path`
-
 /// Correctness of flushing
+
+val mt_flush_to_olds:
+  lv:nat{lv < 32} ->
+  pi:nat ->
+  i:nat{i >= pi} ->
+  j:nat{j >= i /\ j < pow2 (32 - lv)} ->
+  olds:hash_ss{S.length olds = 32 /\ mt_olds_inv lv pi olds} ->
+  hs:hash_ss{S.length hs = 32 /\ hs_wf_elts lv hs pi j} ->
+  GTot (folds:hash_ss{
+         S.length folds = 32 /\
+         S.equal (S.slice olds 0 lv) (S.slice folds 0 lv) /\
+         mt_olds_inv lv i folds})
+       (decreases i)
+let rec mt_flush_to_olds lv pi i j olds hs =
+  let oi = offset_of i in
+  let opi = offset_of pi in
+  if oi = opi then olds (* no updates *)
+  else (let nolds = 
+         S.upd olds lv
+           (S.append (S.index olds lv)
+                     (S.slice (S.index hs lv) 0 (oi - opi))) in
+       mt_olds_inv_equiv (lv + 1) (pi / 2) olds nolds;
+       mt_flush_to_olds (lv + 1) (pi / 2) (i / 2) (j / 2) nolds hs)
+
+val mt_flush_to_olds_hs_equiv:
+  lv:nat{lv < 32} ->
+  pi:nat ->
+  i:nat{i >= pi} ->
+  j:nat{j >= i /\ j < pow2 (32 - lv)} ->
+  olds:hash_ss{S.length olds = 32 /\ mt_olds_inv lv pi olds} ->
+  hs1:hash_ss{S.length hs1 = 32 /\ hs_wf_elts lv hs1 pi j} ->
+  hs2:hash_ss{S.length hs2 = 32 /\ hs_wf_elts lv hs2 pi j} ->
+  Lemma (requires (S.equal (S.slice hs1 lv 32) (S.slice hs2 lv 32)))
+        (ensures (S.equal (mt_flush_to_olds lv pi i j olds hs1)
+                          (mt_flush_to_olds lv pi i j olds hs2)))
+        (decreases i)
+let rec mt_flush_to_olds_hs_equiv lv pi i j olds hs1 hs2 =
+  let oi = offset_of i in
+  let opi = offset_of pi in
+  if oi = opi then ()
+  else (assert (S.index hs1 lv == S.index hs2 lv);
+       let nolds = 
+         S.upd olds lv
+           (S.append (S.index olds lv)
+                     (S.slice (S.index hs1 lv) 0 (oi - opi))) in
+       mt_olds_inv_equiv (lv + 1) (pi / 2) olds nolds;
+       mt_flush_to_olds_hs_equiv
+         (lv + 1) (pi / 2) (i / 2) (j / 2) nolds hs1 hs2)
+
+val mt_flush_to_merge_preserved:
+  lv:nat{lv < 32} ->
+  pi:nat -> i:nat{i >= pi} ->
+  j:nat{j >= i /\ j < pow2 (32 - lv)} ->
+  olds:hash_ss{S.length olds = 32 /\ mt_olds_inv lv pi olds} ->
+  hs:hash_ss{S.length hs = 32 /\ hs_wf_elts lv hs pi j} ->
+  Lemma (requires True)
+        (ensures (S.equal (merge_hs olds hs)
+                          (merge_hs
+                            (mt_flush_to_olds lv pi i j olds hs) 
+                            (mt_flush_to_ lv hs pi i j))))
+        (decreases i)
+#reset-options "--z3rlimit 20 --max_fuel 2"
+let rec mt_flush_to_merge_preserved lv pi i j olds hs =
+  let oi = offset_of i in
+  let opi = offset_of pi in
+  if oi = opi then ()
+  else begin
+    let nolds = S.upd olds lv
+                  (S.append (S.index olds lv)
+                    (S.slice (S.index hs lv) 0 (oi - opi))) in
+    let nhs = S.upd hs lv
+                (S.slice (S.index hs lv) (oi - opi) (j - opi)) in
+    mt_olds_inv_equiv (lv + 1) (pi / 2) olds nolds;
+    hs_wf_elts_equal (lv + 1) hs nhs (pi / 2) (j / 2);
+    mt_flush_to_merge_preserved
+      (lv + 1) (pi / 2) (i / 2) (j / 2) nolds nhs;
+    mt_flush_to_olds_hs_equiv
+      (lv + 1) (pi / 2) (i / 2) (j / 2) nolds hs nhs;
+    assert (S.equal (merge_hs nolds nhs)
+                    (merge_hs
+                      (mt_flush_to_olds lv pi i j olds hs)
+                      (mt_flush_to_ lv hs pi i j)));
+    merge_hs_upd olds hs lv
+      (S.append (S.index olds lv) (S.slice (S.index hs lv) 0 (oi - opi)))
+      (S.slice (S.index hs lv) (oi - opi) (j - opi));
+    assert (S.equal (merge_hs olds hs) (merge_hs nolds nhs))
+  end
+#reset-options
+
+val mt_flush_to_inv_preserved_:
+  lv:nat{lv < 32} ->
+  pi:nat -> i:nat{i >= pi} ->
+  j:nat{j >= i /\ j < pow2 (32 - lv)} ->
+  olds:hash_ss{S.length olds = 32 /\ mt_olds_inv lv pi olds} ->
+  hs:hash_ss{S.length hs = 32 /\ hs_wf_elts lv hs pi j} ->
+  Lemma (requires (mt_olds_hs_inv lv pi j olds hs))
+        (ensures (mt_olds_hs_inv lv i j 
+                   (mt_flush_to_olds lv pi i j olds hs) 
+                   (mt_flush_to_ lv hs pi i j)))
+let mt_flush_to_inv_preserved_ lv pi i j olds hs =
+  mt_flush_to_merge_preserved lv pi i j olds hs;
+  mt_olds_hs_lth_inv_ok lv pi j olds hs;
+  mt_hashes_lth_inv_equiv lv j
+    (merge_hs olds hs)
+    (merge_hs (mt_flush_to_olds lv pi i j olds hs) 
+              (mt_flush_to_ lv hs pi i j));
+  mt_hashes_inv_equiv lv j
+    (merge_hs olds hs)
+    (merge_hs (mt_flush_to_olds lv pi i j olds hs) 
+              (mt_flush_to_ lv hs pi i j))
+
+val mt_flush_to_inv_preserved:
+  mt:merkle_tree{mt_wf_elts mt} ->
+  olds:hash_ss{S.length olds = 32 /\ mt_olds_inv 0 (MT?.i mt) olds} ->
+  idx:nat{idx >= MT?.i mt /\ idx < MT?.j mt} ->
+  Lemma (requires (mt_inv mt olds))
+        (ensures (mt_inv (mt_flush_to mt idx)
+                         (mt_flush_to_olds 0 (MT?.i mt) idx (MT?.j mt) olds (MT?.hs mt))))
+let mt_flush_to_inv_preserved mt olds idx =
+  mt_flush_to_inv_preserved_ 0 (MT?.i mt) idx (MT?.j mt) olds (MT?.hs mt)
+
+val mt_flush_inv_preserved:
+  mt:merkle_tree{mt_wf_elts mt /\ MT?.j mt > MT?.i mt} ->
+  olds:hash_ss{S.length olds = 32 /\ mt_olds_inv 0 (MT?.i mt) olds} ->
+  Lemma (requires (mt_inv mt olds))
+        (ensures (mt_inv (mt_flush mt)
+                         (mt_flush_to_olds
+                           0 (MT?.i mt) (MT?.j mt - 1) (MT?.j mt)
+                           olds (MT?.hs mt))))
+let mt_flush_inv_preserved mt olds =
+  mt_flush_to_inv_preserved mt olds (MT?.j mt - 1)
+
+/// Correctness of `mt_get_root` and `mt_get_path`
 
 /// Correctness of path verification
 
